\documentclass{article}

\usepackage{amsmath}
\usepackage{amssymb}
\usepackage{bbm}
\usepackage[T1]{fontenc}
\usepackage{graphicx}
\usepackage{subfigure}
\usepackage{caption}
\usepackage{float}
\usepackage{geometry}
% \usepackage{nicematrix}
% \usepackage{minted}

\geometry{left = 3.18cm, top = 2.54cm, right = 3.18cm}

\title{\Large\bf MATH 507 Homework 3} 
\author{\normalsize Paul Zhang}
\date{\normalsize\today}

\begin{document}
\maketitle
\small
\section*{Problem 1}
\subsection*{1.1}
We have that 
\begin{align*}
    \mathbb{E}[\mathcal{C}(x)] &= \mathbb{E}\int_0^T \tilde{S}_t x^\prime_t \mathrm{d}t \\
    &= \mathbb{E}\int_0^T S_t x^\prime_t \mathrm{d}t + \eta \mathbb{E}\int_0^T (x^\prime_t)^2 \mathrm{d}t \\
    &= \mathbb{E}\left[(S_Tx_T - S_0x_0) - \int_0^T \sigma X_t \mathrm{d}W_t\right] + \eta \mathbb{E}\int_0^T 
    (x^\prime_t)^2 \mathrm{d}t \\
    &= \mathbb{E}[S_Tx_T] - S_0X + \eta \int_0^T \mathbb{E}[(x^\prime_t)^2] \mathrm{d}t
\end{align*}
Note that Fubini's Theorem is needed for the last step.

\subsection*{1.2}
Define 
$$ J(x) := \mathbb{E}[\mathcal{C}(x) + c x_T^2] $$
and accordingly,
$$ V(t, x) := \inf_{x}J(x) \quad \text{with}\quad V(T, x) = cx^2_T $$
which gives us (assuming $\tau > t$)
\begin{align*}
    V(t, x_t) &= \inf \mathbb{E}\left[S_Tx_T - S_tX_t + \eta \int_t^T (x_s^\prime)^2 \mathrm{d}s \right] \\
    V(\tau, x_\tau) &= \inf \mathbb{E}\left[S_Tx_T - S_\tau X_\tau + \eta \int_\tau^T (x_s^\prime)^2 \mathrm{d}s \right]
\end{align*}
Therefore,
$$ V(t, x_t) = V(\tau, x_\tau) + \inf \mathbb{E}\left[S_\tau x_\tau - S_tX_t + \eta \int_t^\tau (x_s^\prime)^2 \mathrm{d}s\right]$$
The HJB equation is given by 
$$ V_t + \inf [V_x x^\prime + sx^\prime + \eta (x^\prime)^2] = 0 $$
Where $V_t, V_x$ are the time and the space derivative, respectively. Note that the $V_xx$ term is gone since $x$ is 
not a function of $W_t$.

\subsection*{1.3}
Based on the ansatz, the partial derivatives are given by
\begin{align*}
    V_t &= \alpha^\prime_t s^2 + \beta^\prime_t xs + \gamma^\prime_t x^2 + \delta^\prime_t \\
    V_x &= \beta_t s + 2\gamma_t x 
\end{align*}
Plugging the derivatives into the HJB equation gives that 
$$ \alpha^\prime_t s^2 + \beta^\prime_t xs + \gamma^\prime_t x^2 + \delta^\prime_t + 
\inf \left[(\beta_t s + 2\gamma_t x)x^\prime + sx^\prime + \eta (x^\prime)^2\right] = 0 $$
Note that the infimum is quadratic \textit{w.r.t.} $x^\prime$. Therefore,
\begin{equation} x^\prime_{opt} = -\frac{1}{2\eta}(\beta s + s + 2\gamma x) \label{eqn:1.1} \end{equation}
Substitute $x^\prime_{opt}$ into the HJB equation:
\begin{gather*}
    \alpha^\prime_t s^2 + \beta^\prime_t xs + \gamma^\prime_t x^2 + \delta^\prime_t -\frac{1}{4\eta^2}(\beta s + s 
    + 2\gamma x) = 0
\end{gather*}
Thus
\begin{equation*}
    \left\{ \begin{matrix}
    \alpha^\prime s^2 - \frac{1}{4\eta}(\beta + 1)^2 + \delta^\prime = 0 \\
    \beta^\prime s - \frac{1}{\eta} [\gamma s(\beta + 1)] = 0 \\
    \gamma^\prime - \frac{\gamma^2}{\eta} = 0
    \end{matrix} \right.
\end{equation*}
Since we have the terminal condition $V(T, x) = cx^2_T$, we can deduce that $\alpha_T = \beta_T = \delta_T = 0$, 
$\gamma_T = c$, which which we can solved the ODE's above. It turns out that 
\begin{equation*}
    \left\{ \begin{matrix}
        \alpha_t &= 0 \\
        \beta_t &= \frac{T - t}{t - \frac{\eta}{c} - T} \\
        \gamma_t &= \frac{\eta}{T + \frac{\eta}{c} - t} \\
        \delta_t &= -\frac{1}{4\eta}\frac{T - t}{t - \frac{\eta}{c} - T}
    \end{matrix} \right.
\end{equation*}
Now substitute $\alpha, \beta, \gamma, \delta$ into Equation \ref{eqn:1.1}:
$$ (t - \frac{\eta}{c} - T)x^\prime - x = \frac{s}{2c} $$
Fix $x_t = x$, and the solution is given by ($\tau > t$)
$$ x_\tau = \frac{s}{2c}\frac{\tau - t}{t - \frac{\eta}{c} - T} + x\frac{\tau - \frac{\eta}{c} - T}{t - \frac{\eta}
{c} - T} $$

\subsection*{1.4}
Send $c \to \infty$. We have that $x_\tau = x\frac{T - \tau}{T}$, which apparently satisfies the boundary conditions.

\end{document}